code/mpfr/MPFR.Lib.fst
@@ -40,15 +40,17 @@ noeq type mpfr_struct = {
     mpfr_d: buffer mp_limb_t
 }
 
-type mpfr_ptr = b:buffer mpfr_struct{length b = 1}
-type mpfr_srcptr = mpfr_ptr
-
 inline_for_extraction let mk_mpfr_struct p s e d = {
     mpfr_prec = p;
     mpfr_sign = s;
     mpfr_exp = e;
     mpfr_d = d
 }
+
+type mpfr_ptr = b:buffer mpfr_struct{length b = 1}
+type mpfr_srcptr = mpfr_ptr
+
+let as_struct h (a:mpfr_ptr) = Seq.index (as_seq h a) 0
 
 (* range settings *)
 (* precision *)
@@ -86,26 +88,35 @@ let mpfr_d_valn_cond (m:mp_limb_t): GTot Type0 =
 let mpfr_d_val0_cond (m:mp_limb_t) (p:mpfr_prec_t{U32.v p > 0}): GTot Type0 =
     v m % pow2 (prec_to_len (U32.v p) - U32.v p) = 0
 
+let prec_len_cond_ h (s:mpfr_struct): GTot Type0 =
+    prec_to_len (U32.v s.mpfr_prec) = length s.mpfr_d * 64
+
+let prec_len_cond h (a:mpfr_ptr): GTot Type0 = prec_len_cond_ h (as_struct h a)
+
 let normal_cond_ h (s:mpfr_struct): GTot Type0 =
-    prec_to_len (U32.v s.mpfr_prec) = length s.mpfr_d * 64 /\
+    prec_len_cond_ h s /\
     mpfr_d_valn_cond (get h s.mpfr_d (length s.mpfr_d - 1)) /\
     mpfr_d_val0_cond (get h s.mpfr_d 0) s.mpfr_prec
 
-let normal_cond h (a:mpfr_ptr): GTot Type0 = normal_cond_ h (Seq.index (as_seq h a) 0)
+let normal_cond h (a:mpfr_ptr): GTot Type0 = normal_cond_ h (as_struct h a)
+
+let singular_cond_ h (s:mpfr_struct): GTot Type0 =
+    prec_len_cond_ h s /\
+    (s.mpfr_exp = mpfr_EXP_NAN \/ s.mpfr_exp = mpfr_EXP_INF \/ s.mpfr_exp = mpfr_EXP_ZERO)
+
+let singular_cond h (a:mpfr_ptr): GTot Type0 = singular_cond_ h (as_struct h a)
 
 let mpfr_reg_cond_ h (s:mpfr_struct): GTot Type0 =
     normal_cond_ h s /\
     mpfr_PREC_COND (U32.v s.mpfr_prec) /\ mpfr_EXP_COND (I32.v s.mpfr_exp)
 
-let mpfr_reg_cond h (a:mpfr_ptr): GTot Type0 = mpfr_reg_cond_ h (Seq.index (as_seq h a) 0)
+let mpfr_reg_cond h (a:mpfr_ptr): GTot Type0 = mpfr_reg_cond_ h (as_struct h a)
 
 let mpfr_valid_cond_ h (s:mpfr_struct): GTot Type0 =
     mpfr_PREC_COND (U32.v s.mpfr_prec) /\ 
-    prec_to_len (U32.v s.mpfr_prec) = length s.mpfr_d * 64 /\
-    (s.mpfr_exp = mpfr_EXP_NAN \/ s.mpfr_exp = mpfr_EXP_INF \/
-    s.mpfr_exp = mpfr_EXP_ZERO \/ mpfr_reg_cond_ h s)
+    (singular_cond_ h s \/ mpfr_reg_cond_ h s)
 
-let mpfr_valid_cond h (a:mpfr_ptr): GTot Type0 = mpfr_valid_cond_ h (Seq.index (as_seq h a) 0)
+let mpfr_valid_cond h (a:mpfr_ptr): GTot Type0 = mpfr_valid_cond_ h (as_struct h a)
 
 
 (* Conversion to pure struct *)
@@ -133,8 +144,7 @@ let rec to_val_left_slice_lemma s =
 	let rs = Seq.slice s 1 (Seq.length s) in
         to_val_left_slice_lemma rs;
 	lemma_distr_add_left (pow2 64) (v (Seq.index rs 0)) (to_val (Seq.slice rs 1 (Seq.length rs)));
-	lemma_pow2_mul ((Seq.length s - 2) * 64) 64;
-	to_val_right_slice_lemma (Seq.slice s 0 (Seq.length s - 1))
+	lemma_pow2_mul ((Seq.length s - 2) * 64) 64
     end
 
 val to_val1_lemma: s:Seq.seq u64{Seq.length s = 1} -> Lemma
@@ -168,8 +178,6 @@ let val0_cond_lemma s p =
 let as_val h (b:buffer mp_limb_t) = to_val (as_seq h b)
 
 (* Convert valid mpfr_ptr to mpfr_fr *)
-let as_struct h (a:mpfr_ptr) = Seq.index (as_seq h a) 0
-
 val as_normal_: h:mem -> s:mpfr_struct{normal_cond_ h s} -> GTot normal_fp
 
 let as_normal_ h s =
@@ -226,7 +234,7 @@ inline_for_extraction val mpfr_PREC: x:mpfr_ptr -> Stack mpfr_prec_t
     (requires (fun h -> mpfr_live h x))
     (ensures  (fun h0 r h1 -> mpfr_live h1 x /\ h0 == h1 /\
                           r = (as_struct h1 x).mpfr_prec))
-inline_for_extraction let mpfr_PREC x = 
+let mpfr_PREC x = 
     let f = x.(0ul) in
     f.mpfr_prec
 
@@ -234,7 +242,7 @@ inline_for_extraction val mpfr_GET_PREC: x:mpfr_ptr -> Stack mpfr_reg_prec_t
     (requires (fun h -> mpfr_live h x /\ mpfr_PREC_COND (U32.v (as_struct h x).mpfr_prec)))
     (ensures  (fun h0 r h1 -> mpfr_live h1 x /\ h0 == h1 /\
                           r = (as_struct h1 x).mpfr_prec))
-inline_for_extraction let mpfr_GET_PREC x =
+let mpfr_GET_PREC x =
     let f = x.(0ul) in
     f.mpfr_prec
 
@@ -243,7 +251,7 @@ inline_for_extraction val mpfr_EXP: x:mpfr_ptr -> Stack mpfr_exp_t
     (requires (fun h -> mpfr_live h x))
     (ensures  (fun h0 r h1 -> mpfr_live h1 x /\ h0 == h1 /\
                           r = (as_struct h1 x).mpfr_exp))
-inline_for_extraction let mpfr_EXP x = 
+let mpfr_EXP x = 
     (x.(0ul)).mpfr_exp
 
 inline_for_extraction val mpfr_SET_EXP: x:mpfr_ptr -> e:mpfr_exp_t -> Stack unit
@@ -253,7 +261,7 @@ inline_for_extraction val mpfr_SET_EXP: x:mpfr_ptr -> e:mpfr_exp_t -> Stack unit
 			   (as_struct h1 x).mpfr_sign = (as_struct h0 x).mpfr_sign /\
 			   as_seq h1 (as_struct h1 x).mpfr_d == as_seq h0 (as_struct h0 x).mpfr_d))
 
-inline_for_extraction let mpfr_SET_EXP x e = 
+let mpfr_SET_EXP x e = 
     let h0 = ST.get() in
     x.(0ul) <- {x.(0ul) with mpfr_exp = e};
     let h1 = ST.get() in
@@ -274,7 +282,7 @@ inline_for_extraction val mpfr_SIGN: x:mpfr_ptr -> Stack mpfr_sign_t
     (requires (fun h -> mpfr_live h x))
     (ensures  (fun h0 r h1 -> mpfr_live h1 x /\ h0 == h1 /\
                            r = (as_struct h1 x).mpfr_sign))
-inline_for_extraction let mpfr_SIGN x = 
+let mpfr_SIGN x = 
     (x.(0ul)).mpfr_sign
 
 inline_for_extraction val mpfr_SET_SIGN: x:mpfr_ptr -> s:mpfr_sign_t -> Stack unit
@@ -284,7 +292,7 @@ inline_for_extraction val mpfr_SET_SIGN: x:mpfr_ptr -> s:mpfr_sign_t -> Stack un
 			   (as_struct h1 x).mpfr_exp = (as_struct h0 x).mpfr_exp /\
 			   as_seq h1 (as_struct h1 x).mpfr_d == as_seq h0 (as_struct h0 x).mpfr_d))
 			   
-inline_for_extraction let mpfr_SET_SIGN x s = 
+let mpfr_SET_SIGN x s = 
     let h0 = ST.get() in
     x.(0ul) <- {x.(0ul) with mpfr_sign = s};
     let h1 = ST.get() in
@@ -294,18 +302,18 @@ inline_for_extraction let mpfr_SET_SIGN x s =
 inline_for_extraction let mpfr_NEG_SIGN s = if s = mpfr_SIGN_POS then mpfr_SIGN_NEG else mpfr_SIGN_POS
 
 inline_for_extraction val mpfr_IS_POS: x:mpfr_ptr -> Stack bool
-    (requires (fun h -> mpfr_live h x /\ mpfr_valid_cond h x))
-    (ensures  (fun h0 r h1 -> mpfr_live h1 x /\ mpfr_valid_cond h1 x /\ h0 == h1 /\
+    (requires (fun h -> mpfr_live h x /\ (normal_cond h x \/ singular_cond h x)))
+    (ensures  (fun h0 r h1 -> mpfr_live h1 x /\ h0 == h1 /\
                            r = I32.((as_struct h1 x).mpfr_sign >^ 0l)))
 
-inline_for_extraction let mpfr_IS_POS x = I32.(mpfr_SIGN x >^ 0l)
+let mpfr_IS_POS x = I32.(mpfr_SIGN x >^ 0l)
 
 inline_for_extraction val mpfr_IS_NEG: x:mpfr_ptr -> Stack bool
-    (requires (fun h -> mpfr_live h x /\ mpfr_valid_cond h x))
-    (ensures  (fun h0 r h1 -> mpfr_live h1 x /\ mpfr_valid_cond h1 x /\ h0 == h1 /\
+    (requires (fun h -> mpfr_live h x /\ (normal_cond h x \/ singular_cond h x)))
+    (ensures  (fun h0 r h1 -> mpfr_live h1 x /\ h0 == h1 /\
                            r = I32.((as_struct h1 x).mpfr_sign <^ 0l)))
 
-inline_for_extraction let mpfr_IS_NEG x = I32.(mpfr_SIGN x <^ 0l)
+let mpfr_IS_NEG x = I32.(mpfr_SIGN x <^ 0l)
 
 inline_for_extraction let mpfr_IS_STRICTPOS x = mpfr_NOTZERO x /\ mpfr_IS_POS x
 inline_for_extraction let mpfr_IS_STRICTNEG x = mpfr_NOTZERO x /\ mpfr_IS_NEG x
@@ -327,7 +335,7 @@ inline_for_extraction val mpfr_MANT: x:mpfr_ptr -> Stack (buffer mp_limb_t)
     (ensures  (fun h0 r h1 -> mpfr_live h1 x /\ h0 == h1 /\
 			   r == (as_struct h1 x).mpfr_d))
 
-inline_for_extraction let mpfr_MANT x = 
+let mpfr_MANT x = 
     (x.(0ul)).mpfr_d
 
 inline_for_extraction val mpn_ZERO: b:buffer mp_limb_t -> l:u32 -> Stack unit
@@ -338,7 +346,7 @@ inline_for_extraction val mpn_ZERO: b:buffer mp_limb_t -> l:u32 -> Stack unit
         (forall (i:nat{i >= U32.v l /\ i < length b}). Seq.index (as_seq h1 b) i = Seq.index (as_seq h0 b) i) /\
         to_val (Seq.slice (as_seq h1 b) 0 (U32.v l)) = 0))
 
-inline_for_extraction let rec mpn_ZERO b l =
+let rec mpn_ZERO b l =
     if U32.(l =^ 0ul) then () else begin
         b.(U32.(l -^ 1ul)) <- 0uL;
         mpn_ZERO b U32.(l -^ 1ul);
@@ -352,7 +360,7 @@ inline_for_extraction val mpfr_LAST_LIMB: x:mpfr_ptr -> Stack u32
     (ensures  (fun h0 r h1 -> mpfr_live h1 x /\ h0 == h1 /\
                            (U32.v r + 1) * 64 = prec_to_len (U32.v (as_struct h1 x).mpfr_prec)))
 
-inline_for_extraction let mpfr_LAST_LIMB x =
+let mpfr_LAST_LIMB x =
     U32.((mpfr_GET_PREC x -^ 1ul) /^ gmp_NUMB_BITS)
 
 inline_for_extraction val mpfr_LIMB_SIZE: x:mpfr_ptr -> Stack u32
@@ -360,14 +368,14 @@ inline_for_extraction val mpfr_LIMB_SIZE: x:mpfr_ptr -> Stack u32
     (ensures  (fun h0 r h1 -> mpfr_live h1 x /\ h0 == h1 /\
                            U32.v r * 64 = prec_to_len (U32.v (as_struct h1 x).mpfr_prec)))
 
-inline_for_extraction let mpfr_LIMB_SIZE x = U32.(mpfr_LAST_LIMB x +^ 1ul)
+let mpfr_LIMB_SIZE x = U32.(mpfr_LAST_LIMB x +^ 1ul)
 
 (* special value *)
 inline_for_extraction let mpfr_LIMB_ONE = 1uL
 
 inline_for_extraction val mpfr_LIMB_MASK: s:u32{U32.v s < 64} ->
     Tot (r:u64{v r = pow2 (U32.v s) - 1})
-inline_for_extraction let mpfr_LIMB_MASK s =
+let mpfr_LIMB_MASK s =
     lemma_pow2_small_mod (U32.v s) 64;
     (1uL <<^ s) -^ 1uL
 
@@ -377,7 +385,7 @@ inline_for_extraction let mpfr_LIMB_HIGHBIT =
     0x8000000000000000uL
 
 inline_for_extraction val mpfr_LIMB_MAX: s:u64{v s = pow2 64 - 1}
-inline_for_extraction let mpfr_LIMB_MAX =
+let mpfr_LIMB_MAX =
     assert_norm(pow2 64 - 1 = v 0xffffffffffffffffuL);
     0xffffffffffffffffuL
 
@@ -395,7 +403,7 @@ inline_for_extraction val mpfr_setmax_rec: x:mpfr_ptr -> i:u32 -> Stack unit
         v (Seq.index xm 0) = pow2 64 - pow2 (prec_to_len (U32.v p) - U32.v p) /\
         (forall (j:nat{j > 0 /\ j <= U32.v i}). v (Seq.index xm j) = pow2 64 - 1))))
 
-inline_for_extraction let rec mpfr_setmax_rec x i =
+let rec mpfr_setmax_rec x i =
     let mant = mpfr_MANT x in
     if i = 0ul then begin
         let p = mpfr_GET_PREC x in
@@ -431,7 +439,7 @@ let rec to_val_setmax_lemma s sh =
 	to_val_setmax_lemma (Seq.slice s 0 (Seq.length s - 1)) sh
     end
 
-inline_for_extraction val mpfr_setmax: x:mpfr_ptr -> Stack unit
+val mpfr_setmax: x:mpfr_ptr -> Stack unit
     (requires (fun h -> 
         let p = (as_struct h x).mpfr_prec in
         let l = U32.((p -^ 1ul) /^ 64ul +^ 1ul) in
@@ -443,7 +451,7 @@ inline_for_extraction val mpfr_setmax: x:mpfr_ptr -> Stack unit
 	as_reg_fp h1 x == mpfr_max_value (as_reg_fp h1 x).sign (as_reg_fp h1 x).prec /\
 	eval_abs (as_reg_fp h1 x) =. mpfr_overflow_bound (as_reg_fp h1 x).prec))
 
-inline_for_extraction let mpfr_setmax x =
+let mpfr_setmax x =
     mpfr_SET_EXP x mpfr_EMAX;
     mpfr_setmax_rec x (mpfr_LAST_LIMB x);
     let h = ST.get() in
@@ -473,7 +481,7 @@ let rec to_val_setmin_lemma s =
 	to_val_setmin_lemma (Seq.slice s 1 (Seq.length s))
     end
 
-inline_for_extraction val mpfr_setmin: x:mpfr_ptr -> Stack unit
+val mpfr_setmin: x:mpfr_ptr -> Stack unit
     (requires (fun h -> 
         let p = (as_struct h x).mpfr_prec in
         let l = U32.((p -^ 1ul) /^ 64ul +^ 1ul) in
@@ -485,7 +493,7 @@ inline_for_extraction val mpfr_setmin: x:mpfr_ptr -> Stack unit
 	as_reg_fp h1 x == mpfr_min_value (as_reg_fp h1 x).sign (as_reg_fp h1 x).prec /\
 	eval_abs (as_reg_fp h1 x) =. mpfr_underflow_bound (as_reg_fp h1 x).prec))
 
-inline_for_extraction let mpfr_setmin x =
+let mpfr_setmin x =
     mpfr_SET_EXP x mpfr_EMIN;
     let xn = mpfr_LAST_LIMB x in
     let xp = mpfr_MANT x in
